coq/LLVMGen/Compiler.v
@@ -809,6 +809,7 @@ Definition genPower
     py <- incLocal ;;
     storeid0 <- incVoid ;;
     px <- incLocal ;;
+    xv <- incLocal ;;
     '(nexp, ncode) <- genNExpr n ;;
     let ini := genFloatV initial in
     let init_code := src_nexpcode ++ dst_nexpcode ++ ncode ++ [
@@ -818,6 +819,11 @@ Definition genPower
                                                           (IntType, src_nexpr)]
 
                                     ));
+
+                                  (IId xv, INSTR_Load false TYPE_Double
+                                              (TYPE_Pointer TYPE_Double,
+                                               (EXP_Ident (ID_Local px)))
+                                              (ret 8%Z));
            
                                   (IId py,  INSTR_Op (OP_GetElementPtr
                                                         ytyp (yptyp, (EXP_Ident y))
@@ -837,7 +843,6 @@ Definition genPower
     storeid1 <- incVoid ;;
     void2 <- incVoid ;;
     yv <- incLocal ;;
-    xv <- incLocal ;;
     addVars [(ID_Local xv, TYPE_Double); (ID_Local yv, TYPE_Double)] ;;
     '(fexpr, fexpcode) <- genAExpr f ;;
     dropVars 2 ;;
@@ -845,10 +850,6 @@ Definition genPower
           blk_id    := body_block_id ;
           blk_phis  := [];
           blk_code  := [
-                          (IId xv, INSTR_Load false TYPE_Double
-                                              (TYPE_Pointer TYPE_Double,
-                                               (EXP_Ident (ID_Local px)))
-                                              (ret 8%Z));
                           (IId yv, INSTR_Load false TYPE_Double
                                               (TYPE_Pointer TYPE_Double,
                                                (EXP_Ident (ID_Local py)))
